src/PlutusIR/Semantics/Static/Theorems/Weakening.v
@@ -1,4 +1,4 @@
-Require Import PlutusCert.PlutusIR.
+(* Require Import PlutusCert.PlutusIR.
 
 Require Import PlutusCert.PlutusIR.Semantics.Static.Typing.
 Require Import PlutusCert.Util.List.
@@ -115,4 +115,4 @@ Module Typing.
     all: eassumption.
   Qed.
 
-End Typing.
+End Typing. *)
